\begin{case}
$SA^{T_{1}\rightarrow T_{2}}\;(\lambda x_{1}:T_{1}.e_{A})\rightarrow\lambda x_{2}.(SA^{T_{2}}\;((\lambda x_{1}:T_{1}.e_{A})\;(^{T_{1}}BS\;x_{2})))$ where $(A,B)\in\lbrace H,M\rbrace$

$\Gamma\vdash_{S}SA^{T_{1}\rightarrow T_{2}}\;(\lambda x_{1}:T_{1}.e_{A}):T$ by premise.  $T=TST$ by inversion (Lemma \ref{i}).  $\Gamma\vdash_{A}\lambda x_{1}:T_{1}.e_{A}:T_{1}\rightarrow T_{2}$ by inversion and uniqueness of types (Lemma \ref{uot}).  $\Gamma,x_{2}:TST\vdash_{S}x_{2}:TST$ by inversion.  $\Gamma\vdash_{A}^{T_{1}}BS\;x_{2}:T_{1}[T_{i}/T_{i}^{a}]$ and $\Gamma\vdash_{A}(\lambda x_{1}:T_{1}.e_{A})\;(^{T_{1}}BS\;x_{2}):T_{2}$ by inversion and uniqueness of types.  $\Gamma\vdash_{S}SA^{T_{2}}\;((\lambda x_{1}:T_{1}.e_{A})\;(^{T_{1}}BS\;x_{2})):TST$ and $\Gamma\vdash_{S}\lambda x_{2}.(SA^{T_{2}}\;((\lambda x_{1}:T_{1}.e_{A})\;(^{T_{1}}BS\;x_{2}))):TST$ by inversion.  $\Gamma\vdash_{S}\lambda x_{2}.(SA^{T_{2}}\;((\lambda x_{1}:T_{1}.e_{A})\;(^{T_{1}}BS\;x_{2}))):T$ because $TST=T$.
\end{case}