\begin{case}
$e_{S}=\mathtt{cons}$ $e_{S}^{1}$ $e_{S}^{2}$

$e_{S}^{1}$ is a forced value or $e_{S}^{1}\rightarrow e_{S}^{3}$ or $e_{S}^{1}\rightarrow$ \emph{\textbf{Error}: string} by the induction hypothesis.  If $e_{S}^{1}\rightarrow e_{S}^{3}$ then $\mathtt{cons}$ $e_{S}^{1}$ $e_{S}^{2}\rightarrow\mathtt{cons}$ $e_{S}^{3}$ $e_{S}^{2}$.  If $e_{S}^{1}\rightarrow$ \emph{\textbf{Error}: string} then $\mathtt{cons}$ $e_{S}^{1}$ $e_{S}^{2}\rightarrow$ \emph{\textbf{Error}: string}.  $e_{S}^{2}$ is a forced value or $e_{S}^{2}\rightarrow e_{S}^{4}$ or $e_{S}^{1}\rightarrow$ \emph{\textbf{Error}: string} by the induction hypothesis.  If $e_{S}^{2}\rightarrow e_{S}^{4}$ and $e_{M}^{1}$ is a forced value then $\mathtt{cons}$ $e_{S}^{1}$ $e_{S}^{2}\rightarrow\mathtt{cons}$ $e_{S}^{1}$ $e_{S}^{4}$.  If $e_{S}^{2}\rightarrow$ \emph{\textbf{Error}: string} then $\mathtt{cons}$ $e_{S}^{1}$ $e_{S}^{2}\rightarrow$ \emph{\textbf{Error}: string}.  If $e_{S}^{1}$ and $e_{S}^{2}$ are forced values then $\mathtt{cons}$ $e_{S}^{1}$ $e_{S}^{2}$ is a forced value.
\end{case}