\begin{case}

$e_{S}=\mathtt{force}$ $e_{S}^{1}$

If $e_{S}^{1}\rightarrow e_{S}^{2}$ then $\mathtt{force}$ $e_{S}^{1}\rightarrow\mathtt{force}$ $e_{S}^{2}$.  If $e_{S}^{1}\rightarrow$ \emph{\textbf{Error}: string} then $\mathtt{force}$ $e_{S}^{1}\rightarrow$ \emph{\textbf{Error}: string}.  $e_{S}^{1}$ is a value otherwise.  $\mathtt{force}$ $e_{S}^{1}\rightarrow e_{S}^{1}$ $(e_{S}^{1}\neq SH^{T}$ $e_{H}^{1}$ or $e_{S}^{1}=SH^{[T]}$ $(\mathtt{cons}$ $e_{H}^{1}$ $e_{H}^{2}))$.  If $e_{S}^{1}=SH^{T}$ $e_{H}^{1}$ and $e_{S}^{1}\neq SH^{[T]}$ $(\mathtt{cons}$ $e_{H}^{1}$ $e_{H}^{2})$ then $e_{H}^{1}$ is a value or $e_{H}^{1}\rightarrow e_{H}^{2}$ or $e_{H}^{1}\rightarrow$ \emph{\textbf{Error}: string} by Haskell progress (Theorem \ref{hmps}).  If $e_{H}^{1}\rightarrow e_{H}^{2}$ then $SH^{T}$ $e_{H}^{1}\rightarrow SH^{T}$ $e_{H}^{2}$.  If $e_{H}^{1}\rightarrow$ \emph{\textbf{Error}: string} then $SH^{T}$ $e_{H}^{1}\rightarrow$ \emph{\textbf{Error}: string}.  If $e_{H}^{1}$ is a value then $T$ determines the reduction of $SH^{T}$ $e_{H}^{1}$:

\begin{subcase}

$T=L$

$e_{H}^{1}={^{L}H}S$ $v_{S}$ by canonical forms (Lemma \ref{cf}).  $SH^{L}$ $(^{L}HS$ $v_{S})\rightarrow v_{S}$.

\end{subcase}

\begin{subcase}

$T=N$

$e_{H}^{1}=\overline{n}$ by canonical forms (Lemma \ref{cf}).  $SH^{N}$ $\overline{n}\rightarrow\overline{n}$.

\end{subcase}

\begin{subcase}

$T=[T_{1}]$

$e_{H}^{1}=\mathtt{nil}^{T_{1}[T_{i}/T_{i}^{a}]}$ by canonical forms (Lemma \ref{cf}).  $SH^{T_{1}}$ $\mathtt{nil}^{T_{1}[T_{i}/T_{i}^{a}]}\rightarrow\mathtt{nil}$.

\end{subcase}

\begin{subcase}

$T=T_{1}^{a}$

$SH^{T_{1}^{a}}$ $e_{H}^{1}$ is a value.

\end{subcase}

\begin{subcase}

$T=T_{1}\rightarrow T_{2}$

$e_{H}^{1}=\lambda x_{1}:T_{1}[T_{i}/T_{i}^{a}].e_{H}^{3}$ by canonical forms (Lemma \ref{cf}).  $SH^{T_{1}\rightarrow T_{2}}$ $(\lambda x_{1}:T_{1}[T_{i}/T_{i}^{a}].e_{H}^{3})\rightarrow\lambda x_{2}.(SH^{T_{2}}$ $((\lambda x_{1}:T_{1}[T_{i}/T_{i}^{a}].e_{H}^{3})$ $(^{T_{1}}HS$ $x_{2})))$.

\end{subcase}

\begin{subcase}

$T=\forall X.T_{1}$

$e_{H}^{1}\in\lbrace\Lambda X.e_{H}^{3},{^{\forall X.T_{1}}H}S$ $v_{S}\rbrace$ by canonical forms (Lemma \ref{cf}).  $SH^{\forall X.T_{1}}$ $(\Lambda X.e_{H}^{3})\rightarrow SH^{T_{1}[L/X]}$ $((\Lambda X.e_{H}^{3})$ $\lbrace L\rbrace)$.  $SH^{\forall X.T_{1}}$ $(^{\forall X.T_{1}}HS$ $v_{S})\rightarrow v_{S}$.

\end{subcase}

\end{case}