\begin{case}
\label{ab}
$e_{A}={^{T}A}B^{T}$ $e_{B}^{1}$ where $(A,B,C)\in\lbrace(H,M,v),(M,H,e)\rbrace$

$e_{B}^{1}$ is a value or $e_{B}^{1}\rightarrow e_{B}^{2}$ or $e_{B}^{1}\rightarrow$ \emph{\textbf{Error}:\;string} by the induction hypothesis.  If $e_{B}^{1}$ is a value then $T$ determines its reduction.
\begin{subcase}
$T=N$

$e_{B}^{1}=\overline{n}$ by canonical forms (Lemma \ref{cf}).  $^{N}AB^{N}$ $\overline{n}\rightarrow\overline{n}$.
\end{subcase}
\begin{subcase}
$T=T_{1}\rightarrow T_{2}$

$e_{B}^{1}=\lambda x_{1}:T_{1}.e_{B}^{2}$ by canonical forms (Lemma \ref{cf}).  $^{T_{1}\rightarrow T_{2}}AB^{T_{1}\rightarrow T_{2}}$ $(\lambda x_{1}:T_{1}.e_{B}^{2})\rightarrow\lambda x_{2}:T_{1}[T_{i}/T^{a}_{i}].(^{T_{2}}AB^{T_{2}}$ $((\lambda x_{1}:T_{1}.e_{B}^{2})$ $(^{T_{1}}BA^{T_{1}}$ $x_{2})))$.
\end{subcase}
\begin{subcase}
$T=\forall X.T_{1}$

$e_{B}^{1}\in\lbrace\Lambda X.e_{B}^{2},{^{\forall X.T_{1}}B}S$ $v_{S}\rbrace$ by canonical forms (Lemma \ref{cf}).  If $e_{B}^{1}=\Lambda X.e_{B}^{2}$ then $^{\forall X.T_{1}}AB^{\forall X.T_{1}}$ $(\Lambda X.e_{B}^{2})\rightarrow\Lambda X.(^{T_{1}}AB^{T_{1}}$ $e_{B}^{2})$.  If $e_{B}^{1}={^{\forall X.T_{1}}B}S$ $v_{S}$ then $^{\forall X.T_{1}}AB^{\forall X.T_{1}}$ $(^{\forall X.T_{1}}BS$ $v_{S})\rightarrow{^{\forall X.T_{1}}A}S$ $v_{S}$.
\end{subcase}
\begin{subcase}
$T=[T_{1}]$

If $(A,B)=(H,M)$ then $e_{B}^{1}\in\lbrace\mathtt{cons}$ $v_{M}^{1}$ $v_{M}^{2},\mathtt{nil}^{T_{1}},{^{[T_{1}]}M}H^{[T_{1}]}$ $(\mathtt{cons}$ $e_{H}^{1}$ $e_{H}^{2})\rbrace$ by canonical forms (Lemma \ref{cf}).  If $e_{B}^{1}=\mathtt{cons}$ $v_{M}^{1}$ $v_{M}^{2}$ then $^{[T_{1}]}HM^{[T_{1}]}$ $(\mathtt{cons}$ $v_{M}^{1}$ $v_{M}^{2})\rightarrow\mathtt{cons}$ $(^{T_{1}}HM^{T_{1}}$ $v_{M}^{1})$ $(^{[T_{1}]}HM^{[T_{1}]}$ $v_{M}^{2})]$.  If $e_{B}^{1}=\mathtt{nil}^{T_{1}}$ then $^{[T_{1}]}HM^{[T_{1}]}$ $\mathtt{nil}^{T}\rightarrow\mathtt{nil}^{T}$.  If $e_{B}^{1}={^{[T_{1}]}M}H^{[T_{1}]}$ $(\mathtt{cons}$ $e_{H}^{1}$ $e_{H}^{2})$ then $^{[T_{1}]}HM^{[T_{1}]}$ $(^{[T_{1}]}MH^{[T_{1}]}$ $(\mathtt{cons}$ $e_{H}^{1}$ $e_{H}^{2}))\rightarrow\mathtt{cons}$ $e_{H}^{1}$ $e_{H}^{2}$.

If $(A,B)=(M,H)$ then $e_{B}^{1}\in\lbrace\mathtt{cons}$ $e_{H}^{3}$ $e_{H}^{4},\mathtt{nil}^{T_{1}}\rbrace$ by canonical forms.  If $e_{B}^{1}=\mathtt{cons}$ $e_{H}^{3}$ $e_{H}^{4}$ then $^{[T_{1}]}MH^{[T_{1}]}$ $(\mathtt{cons}$ $e_{H}^{3}$ $e_{H}^{4})$ is a value.  If $e_{B}^{1}=\mathtt{nil}^{T_{1}}$ then $^{[T_{1}]}MH^{[T_{1}]}$ $\mathtt{nil}^{T_{1}}\rightarrow\mathtt{nil}^{T_{1}}$.
\end{subcase}
\begin{subcase}
$T=L$

$e_{B}^{1}={^{L}B}S$ $v_{S}$ by canonical forms (Lemma \ref{cf}).  $^{L}AB^{L}$ $(^{L}BS$ $v_{S})\rightarrow{^{L}A}S$ $v_{S}$.
\end{subcase}
\begin{subcase}
$T=T_{1}^{a}$

Cannot occur because $T_{1}^{a}$ occurs only in $^{T_{1}^{a}}AS$ $e_{S}$.
\end{subcase}
If $e_{B}^{1}\rightarrow e_{B}^{2}$ then $^{T}AB^{T}$ $e_{B}^{1}\rightarrow{^{T}A}B$ $e_{B}^{2}$.  If $e_{B}^{1}\rightarrow$ \emph{\textbf{Error}:\;string} then $^{T}AB^{T}$ $e_{B}^{1}\rightarrow$ \emph{\textbf{Error}:\;string}.
\end{case}