\begin{case}
$e_{S}=f\;e_{S}^{1}$

$e_{S}^{1}$ is a value or $e_{S}^{1}\rightarrow e_{S}^{2}$ or $e_{S}^{1}\rightarrow$ \emph{\textbf{Error}:\;string} by the induction hypothesis.  If $e_{S}^{1}\rightarrow e_{S}^{2}$ then $f\;e_{S}^{1}\rightarrow f\;e_{S}^{2}$.  If $e_{S}^{1}\rightarrow$ \emph{\textbf{Error}:\;string} then $f\;e_{S}^{1}\rightarrow$ \emph{\textbf{Error}:\;string}.  $e_{S}^{1}$ is a value otherwise.  If $e_{S}^{1}=\mathtt{cons}\;e_{S}^{3}\;e_{S}^{4}$ then $\mathtt{hd}\;(\mathtt{cons}\;e_{S}^{3}\;e_{S}^{4})\rightarrow e_{S}^{3}$ and $\mathtt{tl}\;(\mathtt{cons}\;e_{S}^{3}\;e_{S}^{4})\rightarrow e_{S}^{4}$.  If $e_{S}^{1}=\mathtt{nil}$ then $\mathtt{hd}\;\mathtt{nil}\rightarrow\mathtt{wrong}\;\mathrm{``Empty\;list"}$ and $\mathtt{tl}\;\mathtt{nil}\rightarrow\mathtt{nil}$.  If $e_{S}^{1}=SH^{[T]}\;(\mathtt{cons}\;e_{H}^{1}\;e_{H}^{2})$ then $\mathtt{hd}\;(SH^{[T]}\;(\mathtt{cons}\;e_{H}^{1}\;e_{H}^{2}))\rightarrow SH^{T}\;e_{H}^{1}$ and $\mathtt{tl}\;(SH^{[T]}\;(\mathtt{cons}\;e_{H}^{1}\;e_{H}^{2}))\rightarrow SH^{[T]}\;e_{H}^{2}$.  $f\;e_{S}^{1}\rightarrow\mathtt{wrong}\;\mathrm{``Not\;a\;list"}$ otherwise.
\end{case}