\begin{case}
$e_{S}=SA^{T}\;e_{A}^{1}$ where $(A,B)\in\lbrace(H,e),(M,v)\rbrace$

$e_{A}^{1}$ is a value or $e_{A}^{1}\rightarrow e_{A}^{2}$ or $e_{A}^{1}\rightarrow$ \emph{\textbf{Error}:\;string} by the induction hypothesis.  If $e_{A}^{1}$ is a value then $T$ determines its reduction.
\begin{subcase}
$T=N$

$e_{A}^{1}=\overline{n}$ by canonical forms (Lemma \ref{cf}).  $SA^{N}\;\overline{n}\rightarrow\overline{n}$.
\end{subcase}
\begin{subcase}
$T=T_{1}\rightarrow T_{2}$

$e_{A}^{1}=\lambda x_{1}:T_{1}[T_{i}/T_{i}^{a}].e_{A}^{3}$ by canonical forms (Lemma \ref{cf}).  $SA^{T_{1}\rightarrow T_{2}}\;(\lambda x_{1}:T_{1}[T_{i}/T_{i}^{a}].e_{A}^{3})\rightarrow\lambda x_{2}.(SA^{T_{2}}\;((\lambda x_{1}:T_{1}[T_{i}/T_{i}^{a}].e_{A}^{3})\;(^{T_{1}}AS\;x_{2})))$.
\end{subcase}
\begin{subcase}
$T=\forall X_{1}.T_{1}$

$e_{A}^{1}\in\lbrace\Lambda X_{1}.e_{A}^{3},{^{\forall X_{1}.T_{1}}A}S\;v_{S}\rbrace$ by canonical forms (Lemma \ref{cf}).  If $e_{A}^{1}=\Lambda X_{1}.e_{A}^{3}$ then $SA^{\forall X_{1}.T_{1}}\;(\Lambda X_{1}.e_{A}^{3})\rightarrow\Lambda X_{2}.(SA^{T_{1}[X_{2}/X_{1}]}\;((\Lambda X_{1}.e_{A}^{3})\;\lbrace X_{2}\rbrace))$.  If $e_{A}^{1}={^{\forall X_{1}.T_{1}}A}S\;v_{S}$ then it reduces by Case \ref{as}.
\end{subcase}
\begin{subcase}
$T=[T_{1}]$

If $A=H$ then $e_{A}^{1}\in\lbrace\mathtt{cons}\;e_{H}^{1}\;e_{H}^{2},\mathtt{nil}^{T_{1}}\rbrace$ by canonical forms (Lemma \ref{cf}).  If $e_{A}^{1}=\mathtt{cons}\;e_{H}^{1}\;e_{H}^{2}$ then $SA^{[T_{1}]}\;(\mathtt{cons}\;e_{H}^{1}\;e_{H}^{2})$ is a value.  If $A=M$ and $e_{A}^{1}=\mathtt{cons}\;B_{A}^{1}\;B_{A}^{2}$ then $SA^{[T_{1}]}\;(\mathtt{cons}\;B_{A}^{1}\;B_{A}^{2})\rightarrow\mathtt{cons}\;(SA^{T_{1}}\;B_{A}^{1})\;(SA^{[T_{1}]}\;B_{A}^{2})$.  If $e_{A}^{1}=\mathtt{nil}^{T_{1}}$ then $SA^{T_{1}}\;\mathtt{nil}^{T_{1}}\rightarrow\mathtt{nil}$.
\end{subcase}
\begin{subcase}
$T=L$

$e_{A}^{1}={^{L}A}S\;v_{S}$ by canonical forms (Lemma \ref{cf}).  $SA^{L}\;(^{L}AS\;v_{S})\rightarrow v_{S}$.
\end{subcase}
\begin{subcase}
$T=T_{1}^{a}$

$SA^{T_{1}^{a}}\;B_{A}^{3}$ is a value.
\end{subcase}
If $e_{A}^{1}\rightarrow e_{A}^{2}$ then $SA^{T}\;e_{A}^{1}\rightarrow SA^{T}\;e_{A}^{2}$.  If $e_{A}^{1}\rightarrow$ \emph{\textbf{Error}:\;string} then $SA^{T}\;e_{A}^{1}\rightarrow$ \emph{\textbf{Error}:\;string}.
\end{case}