\begin{case}
$e_{S}=SH^{T}\;e_{H}^{1}$

$e_{H}^{1}$ is a value or $e_{H}^{1}\rightarrow e_{H}^{2}$ or $e_{H}^{1}\rightarrow$ \emph{\textbf{Error}:\;string} by the induction hypothesis.  If $e_{H}^{1}$ is a value then $T$ determines its reduction.
\begin{subcase}
$T=N$

$e_{H}^{1}=\overline{n}$ by canonical forms (Lemma \ref{cf}).  $SH^{N}\;\overline{n}\rightarrow\overline{n}$.
\end{subcase}
\begin{subcase}
$T=T_{1}\rightarrow T_{2}$

$e_{H}^{1}=\lambda x_{1}:T_{1}.e_{H}^{3}$ by canonical forms (Lemma \ref{cf}).  $SH^{T_{1}\rightarrow T_{2}}\;(\lambda x_{1}:T_{1}.e_{H}^{3})\rightarrow\lambda x_{2}:T_{1}[T_{i}/T^{a}_{i}].(SH^{T_{2}}\;((\lambda x_{1}:T_{1}.e_{H}^{3})\;(SH^{T_{1}}\;x_{2})))$.
\end{subcase}
\begin{subcase}
$T=\forall X_{1}.T_{1}$

$e_{H}^{1}=\Lambda X_{1}.e_{H}^{3}$ by canonical forms (Lemma \ref{cf}).  $SH^{\forall X_{1}.T_{1}}\;(\Lambda X_{1}.e_{H}^{3})\rightarrow\Lambda X_{2}.(SH^{T_{1}[X_{2}/X_{1}]}\;((\Lambda X_{1}.e_{H}^{3})\;\lbrace X_{2}\rbrace))$.
\end{subcase}
\begin{subcase}
$T=[T_{1}]$

$SH^{[T_{1}]}\;v_{H}$ is a value.
\end{subcase}
\begin{subcase}
$T=L$

$e_{H}^{1}=\,^{L}HS\;v_{S}$ by canonical forms (Lemma \ref{cf}).  $SH^{T}\;(^{L}HS\;v_{S}\rightarrow v_{S}$.
\end{subcase}
\begin{subcase}
$T=T_{1}^{a}$

$SH^{T_{1}^{a}}\;e_{H}^{3}$ is a value.
\end{subcase}
If $e_{H}^{1}\rightarrow e_{H}^{2}$ then $SH^{T}\;e_{H}^{1}\rightarrow SH^{T}\;e_{H}^{2}$.  If $e_{H}^{1}\rightarrow$ \emph{\textbf{Error}:\;string} then $SH^{T}\;e_{H}^{1}\rightarrow$ \emph{\textbf{Error}:\;string}.
\end{case}