\begin{hpn}
\label{hpn}
\onehalfspacing
If $\Gamma\vdash e_{H}:T$ and $e_{H}\rightarrow e_{H}'$ then $\Gamma\vdash e_{H}':T$.
\begin{proof}
By cases on the reduction $e_{H}\rightarrow e_{H}'$.
\begin{hpn-case-1}
$\mathscr{E}[(\lambda x:T_{1}.e_{H}^{1})\;e_{H}^{2}]_{H}\rightarrow\mathscr{E}[e_{H}^{1}[e_{H}^{2}/x]]$

$(\lambda x:T_{1}.e_{H}^{1})\;e_{H}^{2}:T$ by the induction hypothesis and uniqueness of types (Lemma \ref{huot}).  $\lambda x:T_{1}.e_{H}^{1}:T_{1}\rightarrow T$, $e_{H}^{2}:T_{1}$, $\Gamma,x:T_{1}\vdash_{H}x:T_{1}$, and $\Gamma,x:T_{1}\vdash_{H}e_{H}^{1}:T$ by inversion (Lemma \ref{hi}) and uniqueness of types (Lemma \ref{huot}).  $e_{H}^{1}[e_{H}^{2}/x]:T$ by term substitution (Lemma \ref{hts}).
\end{hpn-case-1}
\begin{hpn-case-2}
$\mathscr{E}[(\Lambda X.e_{H})\;\lbrace T\rbrace]_{H}\rightarrow\mathscr{E}[e_{H}[T/X]]$


\end{hpn-case-2}
\begin{hpn-case-3}
$\mathscr{E}[\mathtt{if0}\;\overline{0}\;e_{H}^{1}\;e_{H}^{2}]_{H}\rightarrow\mathscr{E}[e_{H}^{1}]$

\end{hpn-case-3}
\begin{hpn-case-4}
$\mathscr{E}[\mathtt{if0}\;\overline{n}\;e_{H}^{1}\;e_{H}^{2}]_{H}\rightarrow\mathscr{E}[e_{H}^{2}]\;(n\neq0)$

\end{hpn-case-4}
\begin{hpn-case-5}
$\mathscr{E}[+\;\overline{n_{1}}\;\overline{n_{2}}]_{H}\rightarrow\mathscr{E}[\overline{n_{1}+n_{2}}]$

\end{hpn-case-5}
\begin{hpn-case-6}
$\mathscr{E}[-\;\overline{n_{1}}\;\overline{n_{2}}]_{H}\rightarrow\mathscr{E}[\overline{(max(n_{1}-n_{2},0)}]$

\end{hpn-case-6}
\begin{hpn-case-7}
$\mathscr{E}[\mathtt{hd}\;(\mathtt{cons}\;e_{H}^{1}\;e_{H}^{2})]_{H}\rightarrow\mathscr{E}[e_{H}^{1}]$

\end{hpn-case-7}
\begin{hpn-case-8}
$\mathscr{E}[\mathtt{tl}\;(\mathtt{cons}\;e_{H}^{1}\;e_{H}^{2})]_{H}\rightarrow\mathscr{E}[e_{H}^{2}]$

\end{hpn-case-8}
\begin{hpn-case-9}
$\mathscr{E}[\mathtt{fix}\;(\lambda x:T.e_{H})]_{H}\rightarrow\mathscr{E}[e_{H}[(\mathtt{fix}\;(\lambda x:T.e_{H}))/x]]$

\end{hpn-case-9}
\begin{hpn-case-10}
$\mathscr{E}[^{N}HM^{N}\;\overline{n}]_{H}\rightarrow\mathscr{E}[\overline{n}]$

\end{hpn-case-10}
\begin{hpn-case-11}
$\mathscr{E}[^{\forall X_{1}.T}HM^{\forall X_{1}.T}\;(\Lambda X_{1}.e_{M})]_{H}\rightarrow\mathscr{E}[\Lambda X_{2}.(^{T[X_{2}/X_{1}]}HM^{T[X_{2}/X_{1}]}\;((\Lambda X_{1}.e_{M})\;\lbrace X_{2}\rbrace))]$


\end{hpn-case-11}
\begin{hpn-case-12}
$\mathscr{E}[^{T_{1}\rightarrow T_{2}}HM^{T_{1}\rightarrow T_{2}}\;(\lambda x_{1}:T_{1}.e_{M})]_{H}\rightarrow\mathscr{E}[\lambda x_{2}:T_{1}.(^{T_{2}}HM^{T_{2}}\;((\lambda x_{1}:T_{1}.e_{M})\;(^{T_{1}}MH^{T_{1}}\;x_{2})))]$

\end{hpn-case-12}
\begin{hpn-case-13}
$\mathscr{E}[^{[T]}HM^{[T]}\;(\mathtt{cons}\;v_{M}^{1}\;v_{M}^{2})]_{H}\rightarrow\mathscr{E}[\mathtt{cons}\;(^{T}HM^{T}\;v_{M}^{1})\;(^{[T]}HM^{[T]}\;v_{M}^{2})]$

\end{hpn-case-13}
\begin{hpn-case-14}
$\mathscr{E}[^{N}HS\;\overline{n}]_{H}\rightarrow\mathscr{E}[\overline{n}]$

\end{hpn-case-14}
\begin{hpn-case-15}
$\mathscr{E}[^{N}HS\;v_{S}]_{H}\rightarrow\mathscr{E}[^{N}HS\;(\mathtt{wrong}\;\mathrm{``Not\;a\;number"})]\;(v_{S}\neq\overline{n}$ for any $\overline{n})$

\end{hpn-case-15}
\begin{hpn-case-16}
$\mathscr{E}[(^{\forall X.T_{1}}HS\;v_{S})\;\lbrace T_{2}\rbrace]_{H}\rightarrow\mathscr{E}[^{T_{1}[T^{a}_{2}/X]}HS\;v_{S}]$

\end{hpn-case-16}
\begin{hpn-case-17}
$\mathscr{E}[^{T_{1}\rightarrow T_{2}}HS\;(\lambda x_{1}.e_{S})]_{H}\rightarrow\mathscr{E}[\lambda x_{2}:T_{1}[T_{i}/T^{a}_{i}].(^{T_{2}}HS\;((\lambda x_{1}.e_{S})\;(SH^{T_{1}}\;x_{2})))]$

\end{hpn-case-17}
\begin{hpn-case-18}
$\mathscr{E}[^{T_{1}\rightarrow T_{2}}HS\;v_{S}]_{H}\rightarrow\mathscr{E}[^{T_{1}\rightarrow T_{2}}HS\;(\mathtt{wrong}\;\mathrm{``Not\;a\;procedure"})]\;(v_{S}\neq\lambda x.e_{S}$ for any $x$ or $e_{S})$

\end{hpn-case-18}
\begin{hpn-case-19}
$\mathscr{E}[^{T^{a}}HS\;(SH^{T^{a}}\;e_{H})]_{H}\rightarrow\mathscr{E}[e_{H}]$

\end{hpn-case-19}
\begin{hpn-case-20}
$\mathscr{E}[^{T^{a}}HS\;v_{S}]_{H}\rightarrow\mathscr{E}[^{T^{a}}HS\;(\mathtt{wrong}\;\mathrm{``Parametricity\;violated"})]\;(v_{S}\neq SH^{T^{a}}\;e_{H}$ for any $e_{H})$

\end{hpn-case-20}
\begin{hpn-case-21}
$\mathscr{E}[^{[T]}HS\;(\mathtt{cons}\;v_{S}^{1}\;v_{S}^{2})]_{H}\rightarrow\mathscr{E}[\mathtt{cons}\;(^{T}HS\;v_{S}^{1})\;(^{[T]}HS\;v_{S}^{2})]$

\end{hpn-case-21}
\begin{hpn-case-22}
$\mathscr{E}[^{[T]}HS\;v_{S}^{1}]_{H}\rightarrow\mathscr{E}[^{[T]}HS\;(\mathtt{wrong}\;\mathrm{``Not\;a\;list"})]\;(v_{S}^{1}\neq\mathtt{cons}\;v_{S}^{2}\;v_{S}^{3}$ for any $v_{S}^{2}$ or $v_{S}^{3})$

\end{hpn-case-22}
\end{proof}
\end{hpn}