\begin{theorem}
\label{ps}
\onehalfspacing
If $\vdash_{HMS}e_{HMS}:T$ then $e_{HMS}$ is a value or $e_{HMS}\rightarrow e_{HMS}'$ or $e_{HMS}\rightarrow$ \emph{\textbf{Error}:\;string}.
\begin{proof}
By structural induction on $e_{HMS}$.
\begin{case}
$e_{HMS}=x$

Cannot occur because $e_{HMS}$ is closed.
\end{case}
\begin{case}
$e_{HMS}=\overline{n}$

$\overline{n}$ is a value.
\end{case}
\begin{case}
$e_{HM}=\lambda x:T.e_{HM}^{1}$

$\lambda x:T.e_{HM}^{1}$ is a value.
\end{case}
\begin{case}
$e_{S}=\lambda x.e_{S}^{1}$

$\lambda x.e_{S}^{1}$ is a value.
\end{case}
\begin{case}
$e_{HM}=\Lambda X.e_{HM}^{1}$

$\Lambda X.e_{HM}^{1}$ is a value.
\end{case}
\begin{case}
$e_{H}=\mathtt{cons}\;e_{H}^{1}\;e_{H}^{2}$

$\mathtt{cons}\;e_{H}^{1}\;e_{H}^{2}$ is a value.
\end{case}
\begin{case}
$e_{MS}=\mathtt{cons}\;v_{MS}^{1}\;v_{MS}^{2}$

$\mathtt{cons}\;v_{MS}^{1}\;v_{MS}^{2}$ is a value.
\end{case}
\begin{case}
$e_{HM}=\mathtt{nil}^{T}$

$\mathtt{nil}^{T}$ is a value.
\end{case}
\begin{case}
$e_{S}=\mathtt{nil}$

$\mathtt{nil}$ is a value.
\end{case}
\begin{case}
$e_{H}=e_{H}^{1}\;e_{H}^{2}$

$e_{H}^{1}$ is a value or $e_{H}^{1}\rightarrow e_{H}^{3}$ or $e_{H}^{1}\rightarrow$ \emph{\textbf{Error}:\;string} by the induction hypothesis.  If $e_{H}^{1}$ is a value then $e_{H}^{1}:T_{1}\rightarrow T_{2}$ by inversion (Lemma \ref{i}) and uniqueness of types (Lemma \ref{uot}) and $e_{H}^{1}=\lambda x:T_{1}.e_{H}^{4}$ by canonical forms (Lemma \ref{cf}).  $(\lambda x:T_{1}.e_{H}^{4})\;e_{H}^{2}\rightarrow e_{H}^{4}[e_{H}^{2}/x]$.  If $e_{H}^{1}\rightarrow e_{H}^{3}$ then $e_{H}^{1}\;e_{H}^{2}\rightarrow e_{H}^{3}\;e_{H}^{2}$.  If $e_{H}^{1}\rightarrow$ \emph{\textbf{Error}:\;string} then $e_{H}^{1}\;e_{H}^{2}\rightarrow$ \emph{\textbf{Error}:\;string}.
\end{case}
\begin{case}
$e_{M}=e_{M}^{1}\;e_{M}^{2}$

$e_{M}^{1}$ is a value or $e_{M}^{1}\rightarrow e_{M}^{3}$ or $e_{M}^{1}\rightarrow$ \emph{\textbf{Error}:\;string} by the induction hypothesis.  If $e_{M}^{1}$ is a value then $e_{M}^{1}:T_{1}\rightarrow T_{2}$ by inversion (Lemma \ref{i}) and uniqueness of types (Lemma \ref{uot}) and $e_{M}^{1}=\lambda x:T_{1}.e_{M}^{4}$ by canonical forms (Lemma \ref{cf}).  If $e_{M}^{1}\rightarrow e_{M}^{3}$ then $e_{M}^{1}\;e_{M}^{2}\rightarrow e_{M}^{3}\;e_{M}^{2}$.  If $e_{M}^{1}\rightarrow$ \emph{\textbf{Error}:\;string} then $e_{M}^{1}\;e_{M}^{2}\rightarrow$ \emph{\textbf{Error}:\;string}.  $e_{M}^{2}$ is a value or $e_{M}^{2}\rightarrow e_{M}^{5}$ or $e_{M}^{2}\rightarrow$ \emph{\textbf{Error}:\;string} by the induction hypothesis.  If $e_{M}^{2}\rightarrow e_{M}^{5}$ and $e_{M}^{1}$ is a value then $e_{M}^{1}\;e_{M}^{2}\rightarrow e_{M}^{1}\;e_{M}^{5}$.  If $e_{M}^{2}\rightarrow$ \emph{\textbf{Error}:\;string} and $e_{M}^{1}$ is a value then $e_{M}^{1}\;e_{M}^{2}\rightarrow$ \emph{\textbf{Error}:\;string}.  If $e_{M}^{1}$ and $e_{M}^{2}$ are values then $(\lambda x:T_{1}.e_{M}^{4})\;e_{M}^{2}\rightarrow e_{M}^{4}[e_{M}^{2}/x]$.
\end{case}
\begin{case}
$e_{S}=e_{S}^{1}\;e_{S}^{2}$

$e_{S}^{1}$ is a value or $e_{S}^{1}\rightarrow e_{S}^{3}$ or $e_{S}^{1}\rightarrow$ \emph{\textbf{Error}:\;string} by the induction hypothesis.  If $e_{S}^{1}\rightarrow e_{S}^{3}$ then $e_{S}^{1}\;e_{S}^{2}\rightarrow e_{S}^{3}\;e_{S}^{2}$.  If $e_{S}^{1}\rightarrow$ \emph{\textbf{Error}:\;string} then $e_{S}^{1}\;e_{S}^{2}\rightarrow$ \emph{\textbf{Error}:\;string}.  $e_{S}^{2}$ is a value or $e_{S}^{2}\rightarrow e_{S}^{4}$ or $e_{S}^{2}\rightarrow$ \emph{\textbf{Error}:\;string} by the induction hypothesis.  If $e_{S}^{2}\rightarrow e_{S}^{4}$ and $e_{S}^{1}$ is a value then $e_{S}^{1}\;e_{S}^{2}\rightarrow e_{S}^{1}\;e_{S}^{4}$.  If $e_{S}^{2}\rightarrow$ \emph{\textbf{Error}:\;string} and $e_{S}^{1}$ is a value then $e_{S}^{1}\;e_{S}^{2}\rightarrow$ \emph{\textbf{Error}:\;string}.  If $e_{S}^{1}$ and $e_{S}^{2}$ are values then $(\lambda x.e_{S}^{5})\;e_{S}^{2}\rightarrow e_{S}^{5}[e_{S}^{2}/x]$ if $e_{S}^{1}=\lambda x.e_{S}^{5}$ or $e_{S}^{1}\;e_{S}^{2}\rightarrow\mathtt{wrong}\;\mathrm{``Not\;a\;procedure"}$ otherwise.
\end{case}
\begin{case}
$e_{H}=e_{H}^{1}\;\lbrace T_{1}\rbrace$

$e_{H}^{1}$ is a value or $e_{H}^{1}\rightarrow e_{H}^{2}$ or $e_{H}^{1}\rightarrow$ \emph{\textbf{Error}:\;string} by the induction hypothesis.  If $e_{H}^{1}$ is a value then $e_{H}^{1}:\forall X.T_{2}$ by inversion (Lemma \ref{i}) and uniqueness of types (Lemma \ref{uot}) and $e_{H}^{1}=\Lambda X.e_{H}^{3}$ or $e_{H}^{1}=\,^{\forall X.T_{2}}HS\;v_{S}$ by canonical forms (Lemma \ref{cf}).  If $e_{H}^{1}\rightarrow e_{H}^{2}$ then $e_{H}^{1}\;\lbrace T_{1}\rbrace\rightarrow e_{H}^{2}\;\lbrace T_{1}\rbrace$.  If $e_{H}^{1}\rightarrow$ \emph{\textbf{Error}:\;string} then $e_{H}^{1}\;\lbrace T_{1}\rbrace\rightarrow$ \emph{\textbf{Error}:\;string}.
\end{case}
\begin{subcase}
$e_{H}^{1}=\Lambda X.e_{H}^{3}$

$(\Lambda X.e_{H}^{3})\;\lbrace T_{1}\rbrace\rightarrow e_{H}^{3}[T_{1}/X]$.
\end{subcase}
\begin{subcase}
$e_{H}^{1}=\,^{\forall X.T_{2}}HS\;v_{S}$

$(^{\forall X.T_{2}}HS\;v_{S})\;\lbrace T_{1}\rbrace\rightarrow\,^{T_{2}[T_{1}^{a}/X]}HS\;v_{S}$.
\end{subcase}
\begin{case}
$e_{HM}=\mathtt{if0}\;e_{HM}^{1}\;e_{HM}^{2}\;e_{HM}^{3}$

$e_{HM}^{1}$ is a value or $e_{HM}^{1}\rightarrow e_{HM}^{4}$ or $e_{HM}^{1}\rightarrow$ \emph{\textbf{Error}:\;string} by the induction hypothesis.  If $e_{HM}^{1}$ is a value then $e_{HM}^{1}:N$ by inversion (Lemma \ref{i}) and uniqueness of types (Lemma \ref{uot}) and $e_{HM}^{1}=\overline{n}$ by canonical forms (Lemma \ref{cf}).  $\mathtt{if0}\;e_{HM}^{1}\;e_{HM}^{2}\;e_{HM}^{3}\rightarrow e_{HM}^{2}$ if $e_{HM}^{1}=\overline{0}$ or $\mathtt{if0}\;e_{HM}^{1}\;e_{HM}^{2}\;e_{HM}^{3}\rightarrow e_{HM}^{3}$ otherwise.  If $e_{HM}^{1}\rightarrow e_{HM}^{4}$ then $\mathtt{if0}\;e_{HM}^{1}\;e_{HM}^{2}\;e_{HM}^{3}\rightarrow \mathtt{if0}\;e_{HM}^{4}\;e_{HM}^{2}\;e_{HM}^{3}$.  If $e_{HM}^{1}\rightarrow$ \emph{\textbf{Error}:\;string} then $\mathtt{if0}\;e_{HM}^{1}\;e_{HM}^{2}\;e_{HM}^{3}\rightarrow$ \emph{\textbf{Error}:\;string}.
\end{case}
\begin{case}
$e_{S}=\mathtt{if0}\;e_{S}^{1}\;e_{S}^{2}\;e_{S}^{3}$

$e_{S}^{1}$ is a value or $e_{S}^{1}\rightarrow e_{S}^{4}$ or $e_{S}^{1}\rightarrow$ \emph{\textbf{Error}:\;string} by the induction hypothesis.  If $e_{S}^{1}$ is a value then $\mathtt{if0}\;e_{S}^{1}\;e_{S}^{2}\;e_{S}^{3}\rightarrow e_{S}^{2}$ if $e_{S}^{1}=\overline{0}$ or $\mathtt{if0}\;e_{S}^{1}\;e_{S}^{2}\;e_{S}^{3}\rightarrow e_{S}^{3}$ otherwise.  If $e_{S}^{1}\rightarrow e_{S}^{4}$ then $\mathtt{if0}\;e_{S}^{1}\;e_{S}^{2}\;e_{S}^{3}\rightarrow \mathtt{if0}\;e_{S}^{4}\;e_{S}^{2}\;e_{S}^{3}$.  If $e_{S}^{1}\rightarrow$ \emph{\textbf{Error}:\;string} then $\mathtt{if0}\;e_{S}^{1}\;e_{S}^{2}\;e_{S}^{3}\rightarrow$ \emph{\textbf{Error}:\;string}.
\end{case}
\begin{case}
$e_{HM}=o\;e_{HM}^{1}\;e_{HM}^{2}$

$e_{HM}^{1}$ is a value or $e_{HM}^{1}\rightarrow e_{HM}^{3}$ or $e_{HM}^{1}\rightarrow$ \emph{\textbf{Error}:\;string} by the induction hypothesis.  If $e_{HM}^{1}$ is a value then $e_{HM}^{1}:N$ by inversion (Lemma \ref{i}) and uniqueness of types (Lemma \ref{uot}) and $e_{HM}^{1}=\overline{n_{1}}$ by canonical forms (Lemma \ref{cf}).  If $e_{HM}^{1}\rightarrow e_{HM}^{3}$ then $o\;e_{HM}^{1}\;e_{HM}^{2}\rightarrow o\;e_{HM}^{3}\;e_{HM}^{2}$.  If $e_{HM}^{1}\rightarrow$ \emph{\textbf{Error}:\;string} then $o\;e_{HM}^{1}\;e_{HM}^{2}\rightarrow$ \emph{\textbf{Error}:\;string}.  $e_{HM}^{2}$ is a value or $e_{HM}^{2}\rightarrow e_{HM}^{4}$ or $e_{HM}^{2}\rightarrow$ \emph{\textbf{Error}:\;string} by the induction hypothesis.  If $e_{HM}^{2}$ is a value then $e_{HM}^{2}:N$ by inversion (Lemma \ref{i}) and uniqueness of types (Lemma \ref{uot}) and $e_{HM}^{2}=\overline{n_{2}}$ by canonical forms (Lemma \ref{cf}).  If $e_{HM}^{2}\rightarrow e_{HM}^{4}$ and $e_{HM}^{1}$ is a value then $o\;e_{HM}^{1}\;e_{HM}^{2}\rightarrow o\;e_{HM}^{1}\;e_{HM}^{4}$.  If $e_{HM}^{2}\rightarrow$ \emph{\textbf{Error}:\;string} and $e_{HM}^{1}$ is a value then $o\;e_{HM}^{1}\;e_{HM}^{2}\rightarrow$ \emph{\textbf{Error}:\;string}.  If $e_{HM}^{1}=\overline{n_{1}}$ and $e_{HM}^{2}=\overline{n_{2}}$ then $o\;e_{HM}^{1}\;e_{HM}^{2}\rightarrow\overline{n_{1}+n_{2}}$ if $o=+$ or $o\;e_{HM}^{1}\;e_{HM}^{2}\rightarrow\overline{max(n_{1}-n_{2},0)}$ if $o=-$.
\end{case}
\begin{case}
$e_{S}=o\;e_{S}^{1}\;e_{S}^{2}$

$e_{S}^{1}$ is a value or $e_{S}^{1}\rightarrow e_{S}^{3}$ or $e_{S}^{1}\rightarrow$ \emph{\textbf{Error}:\;string} by the induction hypothesis.  If $e_{S}^{1}\rightarrow e_{S}^{3}$ then $o\;e_{S}^{1}\;e_{S}^{2}\rightarrow o\;e_{S}^{3}\;e_{S}^{2}$.  If $e_{S}^{1}\rightarrow$ \emph{\textbf{Error}:\;string} then $o\;e_{S}^{1}\;e_{S}^{2}\rightarrow$ \emph{\textbf{Error}:\;string}.  $e_{S}^{2}$ is a value or $e_{S}^{2}\rightarrow e_{S}^{4}$ or $e_{S}^{2}\rightarrow$ \emph{\textbf{Error}:\;string} by the induction hypothesis.  If $e_{S}^{2}\rightarrow e_{S}^{4}$ and $e_{S}^{1}$ is a value then $o\;e_{S}^{1}\;e_{S}^{2}\rightarrow o\;e_{S}^{1}\;e_{S}^{4}$.  If $e_{S}^{2}\rightarrow$ \emph{\textbf{Error}:\;string} and $e_{S}^{1}$ is a value then $o\;e_{S}^{1}\;e_{S}^{2}\rightarrow$ \emph{\textbf{Error}:\;string}.  If $e_{S}^{1}$ and $e_{S}^{2}$ are values then $o\;e_{S}^{1}\;e_{S}^{2}\rightarrow\overline{n_{1}+n_{2}}$ if $o=+$, $e_{S}^{1}=\overline{n_{1}}$, and $e_{S}^{2}=\overline{n_{2}}$ and $o\;e_{S}^{1}\;e_{S}^{2}\rightarrow\overline{max(n_{1}-n_{2},0)}$ if $o=-$, $e_{S}^{1}=\overline{n_{1}}$, and $e_{S}^{2}=\overline{n_{2}}$ and $o\;e_{S}^{1}\;e_{S}^{2}\rightarrow\mathtt{wrong}\;\mathrm{``Not\;a\;number"}$ otherwise.
\end{case}
\begin{case}
$e_{H}=f\;e_{H}^{1}$

$e_{H}^{1}$ is a value or $e_{H}^{1}\rightarrow e_{H}^{2}$ or $e_{H}^{1}\rightarrow$ \emph{\textbf{Error}:\;string} by the induction hypothesis.  If $e_{H}^{1}$ is a value then $e_{H}^{1}:[T]$ by inversion (Lemma \ref{i}) and uniqueness of types (Lemma \ref{uot}) and $e_{H}^{1}=\mathtt{cons}\;e_{H}^{2}\;e_{H}^{3}$ or $e_{H}^{1}=\mathtt{nil}^{T}$ by canonical forms (Lemma \ref{cf}).  If $e_{H}^{1}=\mathtt{cons}\;e_{H}^{2}\;e_{H}^{3}$ then $f\;e_{H}^{1}\rightarrow e_{H}^{2}$ if $f=\mathtt{hd}$ or $f\;e_{H}^{1}\rightarrow e_{H}^{3}$ if $f=\mathtt{tl}$.  If $e_{H}^{1}=\mathtt{nil}^{T}$ then $f\;e_{H}^{1}\rightarrow\,^{T}HS\;(\mathtt{wrong}\;\mathrm{``Empty\;list"})$ if $f=\mathtt{hd}$ or $f\;e_{H}^{1}\rightarrow\mathtt{nil}^{T}$ if $f=\mathtt{tl}$.  If $e_{H}^{1}\rightarrow e_{H}^{2}$ then $f\;e_{H}^{1}\rightarrow f\;e_{H}^{2}$.  If $e_{H}^{1}\rightarrow$ \emph{\textbf{Error}:\;string} then $f\;e_{H}^{1}\rightarrow$ \emph{\textbf{Error}:\;string}.
\end{case}
\begin{case}
$e_{M}=f\;e_{M}^{1}$

$e_{M}^{1}$ is a value or $e_{M}^{1}\rightarrow e_{M}^{2}$ or $e_{M}^{1}\rightarrow$ \emph{\textbf{Error}:\;string} by the induction hypothesis.  If $e_{M}^{1}$ is a value then $e_{M}^{1}:[T]$ by inversion (Lemma \ref{i}) and uniqueness of types (Lemma \ref{uot}) and $e_{M}^{1}=\mathtt{cons}\;e_{M}^{2}\;e_{M}^{3}$ or $e_{M}^{1}=\mathtt{nil}^{T}$ or $e_{M}^{1}=\,^{[T]}MH^{[T]}\;v_{H}$ by canonical forms (Lemma \ref{cf}).  If $e_{M}^{1}=\mathtt{cons}\;e_{M}^{2}\;e_{M}^{3}$ then $f\;e_{M}^{1}\rightarrow e_{M}^{2}$ if $f=\mathtt{hd}$ or $f\;e_{M}^{1}\rightarrow e_{M}^{3}$ if $f=\mathtt{tl}$.  If $e_{M}^{1}=\mathtt{nil}^{T}$ then $f\;e_{M}^{1}\rightarrow\,^{T}MS\;(\mathtt{wrong}\;\mathrm{``Empty\;list"})$ if $f=\mathtt{hd}$ or $f\;e_{M}^{1}\rightarrow\mathtt{nil}^{T}$ if $f=\mathtt{tl}$.  If $e_{M}^{1}=\,^{[T]}MH^{[T]}\;v_{H}$ then $v_{H}:[T]$ by inversion (Lemma \ref{i}) and uniqueness of types (Lemma \ref{uot}) and $v_{H}=\mathtt{cons}\;e_{H}^{1}\;e_{H}^{2}$ or $v_{H}=\mathtt{nil}^{T}$ by canonical forms (Lemma \ref{cf}).  If $v_{H}=\mathtt{cons}\;e_{H}^{1}\;e_{H}^{2}$ then $f\;e_{M}^{1}\rightarrow\,^{T}MH^{T}\;e_{H}^{1}$ if $f=\mathtt{hd}$ and $f\;e_{M}^{1}\rightarrow\,^{[T]}MH^{[T]}\;e_{H}^{2}$ if $f=\mathtt{tl}$.  If $v_{H}=\mathtt{nil}^{T}$ then $f\;e_{M}^{1}\rightarrow\,^{T}MS\;(\mathtt{wrong}\;\mathrm{``Empty\;list"})$ if $f=\mathtt{hd}$ and $f\;e_{M}^{1}\rightarrow\mathtt{nil}^{T}$ if $f=\mathtt{tl}$.  If $e_{M}^{1}\rightarrow e_{M}^{2}$ then $f\;e_{M}^{1}\rightarrow f\;e_{M}^{2}$.  If $e_{M}^{1}\rightarrow e_{M}^{2}$ then $f\;e_{M}^{1}\rightarrow f\;e_{M}^{2}$.  If $e_{M}^{1}\rightarrow$ \emph{\textbf{Error}:\;string} then $f\;e_{M}^{1}\rightarrow$ \emph{\textbf{Error}:\;string}.
\end{case}
\begin{case}
$e_{S}=f\;e_{S}^{1}$

$e_{S}^{1}$ is a value or $e_{S}^{1}\rightarrow e_{S}^{2}$ or $e_{S}^{1}\rightarrow$ \emph{\textbf{Error}:\;string} by the induction hypothesis.  If $e_{S}^{1}=\mathtt{cons}\;e_{S}^{2}\;e_{S}^{3}$ then $f\;e_{S}^{1}\rightarrow e_{S}^{2}$ if $f=\mathtt{hd}$ or $f\;e_{S}^{1}\rightarrow e_{S}^{3}$ if $f=\mathtt{tl}$.  If $e_{S}^{1}=\mathtt{nil}$ then $f\;e_{S}^{1}\rightarrow\mathtt{wrong}\;\mathrm{``Empty\;list"}$ if $f=\mathtt{hd}$ or $f\;e_{S}^{1}\rightarrow\mathtt{nil}$ if $f=\mathtt{tl}$.  If $e_{S}^{1}=SH^{[T]}\;v_{H}$ then $v_{H}:[T]$ by inversion (Lemma \ref{i}) and uniqueness of types (Lemma \ref{uot}) and $v_{H}=\mathtt{cons}\;e_{H}^{1}\;e_{H}^{2}$ or $v_{H}=\mathtt{nil}^{T}$ by canonical forms (Lemma \ref{cf}).  If $v_{H}=\mathtt{cons}\;e_{H}^{1}\;e_{H}^{2}$ then $f\;e_{S}^{1}\rightarrow SH^{T}\;e_{H}^{1}$ if $f=\mathtt{hd}$ and $f\;e_{S}^{1}\rightarrow SH^{[T]}\;e_{H}^{2}$ if $f=\mathtt{tl}$.  If $v_{H}=\mathtt{nil}^{T}$ then $f\;e_{S}^{1}\rightarrow\mathtt{wrong}\;\mathrm{``Empty\;list"}$ if $f=\mathtt{hd}$ and $f\;e_{S}^{1}\rightarrow\mathtt{nil}$ if $f=\mathtt{tl}$.  Otherwise $f\;e_{S}^{1}\rightarrow\mathtt{wrong}\;\mathrm{``Not\;a\;list"}$.  If $e_{S}^{1}\rightarrow e_{S}^{2}$ then $f\;e_{S}^{1}\rightarrow f\;e_{S}^{2}$.  If $e_{S}^{1}\rightarrow e_{S}^{2}$ then $f\;e_{S}^{1}\rightarrow f\;e_{S}^{2}$.  If $e_{S}^{1}\rightarrow$ \emph{\textbf{Error}:\;string} then $f\;e_{S}^{1}\rightarrow$ \emph{\textbf{Error}:\;string}.
\end{case}
\begin{case}
$e_{H}=\mathtt{fix}\;e_{H}^{1}$

By the induction hypothesis, either $e_{H}^{1}$ is a value, $e_{H}^{1}\rightarrow e_{H}^{2}$ for some $e_{H}^{2}$, or $e_{H}^{1}\rightarrow$ \emph{\textbf{Error}:\;string} for some \emph{string}.  If $e_{H}^{1}$ is a value then $e_{H}^{1}:T_{1}\rightarrow T_{2}$ for some $T_{1}$ and $T_{2}$ by inversion (Lemma \ref{i}) and uniqueness of types (Lemma \ref{uot}) and $e_{H}^{1}=\lambda x:T_{1}.e_{H}^{2}$ for some $x$ and $e_{H}^{2}$ by canonical forms (Lemma \ref{cf}).  Therefore $\mathtt{fix}\;(\lambda x:T_{1}.e_{H}^{2})\rightarrow e_{H}^{2}[\mathtt{fix}\;(\lambda x:T_{1}.e_{H}^{2})/x]$.  If $e_{H}^{1}\rightarrow e_{H}^{2}$ for some $e_{H}^{2}$ then $\mathtt{fix}\;e_{H}^{1}\rightarrow\mathtt{fix}\;e_{H}^{2}$.  If $e_{H}^{1}\rightarrow$ \emph{\textbf{Error}:\;string} for some \emph{string} then $\mathtt{fix}\;e_{H}^{1}\rightarrow$ \emph{\textbf{Error}:\;string}.
\end{case}
\begin{case}
$e_{H}=\,^{T}HM^{T}\;e_{M}^{1}$

By the ML progress theorem (Theorem \ref{mps}), either $e_{M}^{1}\rightarrow e_{M}^{2}$ for some $e_{M}^{2}$, $e_{M}^{1}\rightarrow$ \emph{\textbf{Error}:\;string} for some \emph{string}, or $e_{M}^{1}$ is a value.  If $e_{M}^{1}\rightarrow e_{M}^{2}$ for some $e_{M}^{2}$ then $^{T}HS\;e_{M}^{1}\rightarrow\,^{T}HS\;e_{M}^{2}$.  If $e_{M}^{1}\rightarrow$ \emph{\textbf{Error}:\;string} for some \emph{string} then $^{T}HS\;e_{M}^{1}\rightarrow$ \emph{\textbf{Error}:\;string}.  If $e_{M}^{1}$ is a value then $T$ determines its reduction:
\begin{case}
$T=N$

$e_{M}^{1}=\overline{n}$ for some $\overline{n}$ by canonical forms (Lemma \ref{mcf}).  $^{N}HM^{N}\;\overline{n}\rightarrow\overline{n}$.
\end{case}
\begin{case}
$T=T_{1}\rightarrow T_{2}$

$e_{M}^{1}=\lambda x_{1}:T_{1}.e_{M}^{2}$ for some $x_{1}$ and $e_{M}^{2}$ by canonical forms (Lemma \ref{mcf}).  $^{T_{1}\rightarrow T_{2}}HM^{T_{1}\rightarrow T_{2}}\;(\lambda x_{1}:T_{1}.e_{M}^{2})\rightarrow\lambda x_{2}:T_{1}[T_{i}/T^{a}_{i}].(^{T_{2}}HM^{T_{2}}\;((\lambda x_{1}:T_{1}.e_{M}^{2})\;(^{T_{1}}MH^{T_{1}}\;x_{2})))$.
\end{case}
\begin{case}
$T=\forall X_{1}.T_{1}$

$e_{M}^{1}=\Lambda X_{1}.e_{M}^{2}$ for some $e_{M}^{2}$ by canonical forms (Lemma \ref{mcf}).  $^{\forall X_{1}.T_{1}}HM^{\forall X_{1}.T_{1}}\;(\Lambda X_{1}.e_{M}^{2})\rightarrow\Lambda X_{2}.(^{T_{1}[X_{2}/X_{1}]}HM^{T_{1}[X_{2}/X_{1}]}\;((\Lambda X_{1}.e_{M}^{2})\;\lbrace X_{2}\rbrace))$.
\end{case}
\begin{case}
$T=[T_{1}]$

$e_{M}^{1}=\mathtt{cons}\;v_{M}^{1}\;v_{M}^{2}$ for some $v_{M}^{1}$ and $v_{M}^{1}$ by canonical forms (Lemma \ref{mcf}).  $^{[T_{1}]}HM^{[T_{1}]}\;(\mathtt{cons}\;v_{M}^{1}\;v_{M}^{2})\rightarrow\mathtt{cons}\;(^{T_{1}}HM^{T_{1}}\;v_{M}^{1})\;(^{[T_{1}]}HM^{[T_{1}]}\;v_{M}^{2})$.
\end{case}
\begin{case}
$T=L$

Cannot occur because $L$ occurs only in $^{L}HS\;e_{S}$.
\end{case}
\begin{case}
$T=T_{1}^{a}$

Cannot occur because $T_{1}^{a}$ occurs only in $^{T_{1}^{a}}HS\;e_{S}$.
\end{case}
\end{case}
\begin{case}
$e_{H}=\,^{T}HS\;e_{S}^{1}$

By the Scheme progress theorem (Theorem \ref{sps}), either $e_{S}^{1}\rightarrow e_{S}^{2}$ for some $e_{S}^{2}$, $e_{S}^{1}\rightarrow$ \emph{\textbf{Error}:\;string} for some \emph{string}, or $e_{S}^{1}$ is a value.  If $e_{S}^{1}\rightarrow e_{S}^{2}$ for some $e_{S}^{2}$ then $^{T}HS\;e_{S}^{1}\rightarrow\,^{T}HS\;e_{S}^{2}$.  If $e_{S}^{1}\rightarrow$ \emph{\textbf{Error}:\;string} for some \emph{string} then $^{T}HS\;e_{S}^{1}\rightarrow$ \emph{\textbf{Error}:\;string}.  If $e_{S}^{1}$ is a value then $T$ determines its reduction:
\begin{case}
$T=N$

If $e_{S}^{1}=\overline{n}$ for some $\overline{n}$ then $^{N}HS\;\overline{n}\rightarrow\overline{n}$.  Otherwise, $^{N}HS\;e_{S}^{1}\rightarrow\,^{N}HS\;(\mathtt{wrong}\;\mathrm{``Not\;a\;number"})$.
\end{case}
\begin{case}
$T=T_{1}\rightarrow T_{2}$

If $e_{S}^{1}=\lambda x_{1}.e_{S}^{2}$ for some $x_{1}$ and $e_{S}^{2}$ then $^{T_{1}\rightarrow T_{2}}HS\;(\lambda x_{1}.e_{S}^{2})\rightarrow\lambda x_{2}:T_{1}[T_{i}/T^{a}_{i}].(^{T_{2}}HS\;((\lambda x_{1}.e_{S}^{2})\;(SH^{T_{1}}\;x_{2})))$.  Otherwise, $^{T_{1}\rightarrow T_{2}}HS\;e_{S}^{1}\rightarrow\,^{T_{1}\rightarrow T_{2}}HS\;(\mathtt{wrong}\;\mathrm{``Not\;a\;procedure"})$.
\end{case}
\begin{case}
$T=\forall X.T_{1}$

$^{\forall X.T_{1}}HS\;e_{S}^{1}$ is a value.
\end{case}
\begin{case}
$T=[T_{1}]$

If $e_{S}^{1}=\mathtt{cons}\;v_{S}^{2}\;v_{S}^{3}$ for some $v_{S}^{2}$ and $v_{S}^{3}$ then $^{[T_{1}]}HS\;(\mathtt{cons}\;v_{S}^{2}\;v_{S}^{3})\rightarrow\mathtt{cons}\;(^{T_{1}}HS\;v_{S}^{2})\;(^{[T_{1}]}HS\;v_{S}^{3})$.  Otherwise, $^{[T_{1}]}HS\;e_{S}^{1}\rightarrow\,^{[T_{1}]}HS\;(\mathtt{wrong}\;\mathrm{``Not\;a\;list"})$.
\end{case}
\begin{case}
$T=L$

$^{L}HS\;e_{S}^{1}$ is a value.
\end{case}
\begin{case}
$T=T_{1}^{a}$

If $e_{S}^{1}=SH^{T_{1}^{a}}\;e_{H}^{1}$ then $^{T_{1}^{a}}HS\;(SH^{T_{1}^{a}}\;e_{H}^{1})\rightarrow e_{H}^{1}$.  Otherwise, $^{T_{1}^{a}}HS\;e_{S}^{1}\rightarrow\,^{T_{1}^{a}}HS\;(\mathtt{wrong}\;\mathrm{``Parametricity\;violated"})$.
\end{case}
\end{case}
\end{proof}
\end{theorem}