\begin{case}
$e_{H}=e_{H}^{1}\;\lbrace T_{1}\rbrace$

$e_{H}^{1}$ is a value or $e_{H}^{1}\rightarrow e_{H}^{2}$ or $e_{H}^{1}\rightarrow$ \emph{\textbf{Error}:\;string} by the induction hypothesis.  If $e_{H}^{1}$ is a value then $e_{H}^{1}:\forall X.T_{2}$ by inversion (Lemma \ref{i}) and uniqueness of types (Lemma \ref{uot}) and $e_{H}^{1}=\Lambda X.e_{H}^{3}$ or $e_{H}^{1}=\,^{\forall X.T_{2}}HS\;v_{S}$ by canonical forms (Lemma \ref{cf}).
\begin{subcase}
$e_{H}^{1}=\Lambda X.e_{H}^{3}$

$(\Lambda X.e_{H}^{3})\;\lbrace T_{1}\rbrace\rightarrow e_{H}^{3}[T_{1}/X]$.
\end{subcase}
\begin{subcase}
$e_{H}^{1}=\,^{\forall X.T_{2}}HS\;v_{S}$

$(^{\forall X.T_{2}}HS\;v_{S})\;\lbrace T_{1}\rbrace\rightarrow\,^{T_{2}[T_{1}^{a}/X]}HS\;v_{S}$.
\end{subcase}
If $e_{H}^{1}\rightarrow e_{H}^{2}$ then $e_{H}^{1}\;\lbrace T_{1}\rbrace\rightarrow e_{H}^{2}\;\lbrace T_{1}\rbrace$.  If $e_{H}^{1}\rightarrow$ \emph{\textbf{Error}:\;string} then $e_{H}^{1}\;\lbrace T_{1}\rbrace\rightarrow$ \emph{\textbf{Error}:\;string}.
\end{case}