\begin{theorem}
\label{pn}
\onehalfspacing
If $\Gamma\vdash_{HMS}e_{HMS}^{1}:T$ and $e_{HMS}^{1}\rightarrow e_{HMS}^{2}$ then $\Gamma\vdash_{HMS}e_{HMS}^{2}:T$.
\begin{proof}
By cases on the reduction $e_{HMS}^{1}\rightarrow e_{HMS}^{2}$.  Scheme reductions that do not contain Haskell or ML terms are omitted because demonstrating the preservation of $TST$ is straightforward.
\input{cases/preservation/term-application.tex}
\input{cases/preservation/type-application.tex}
\input{cases/preservation/if-true.tex}
\input{cases/preservation/if-false.tex}
\input{cases/preservation/addition.tex}
\input{cases/preservation/subtraction.tex}
\input{cases/preservation/head-cons.tex}
\input{cases/preservation/tail-cons.tex}
\input{cases/preservation/head-nil.tex}
\input{cases/preservation/tail-nil.tex}
\input{cases/preservation/fix.tex}
%\input{cases/preservation/.tex}

\begin{case}
$\mathscr{E}[^{N}HM^{N}\;\overline{n}]_{H}\rightarrow\mathscr{E}[\overline{n}]$

\end{case}
\begin{case}
$\mathscr{E}[^{\forall X_{1}.T}HM^{\forall X_{1}.T}\;(\Lambda X_{1}.e_{M})]_{H}\rightarrow\mathscr{E}[\Lambda X_{2}.(^{T[X_{2}/X_{1}]}HM^{T[X_{2}/X_{1}]}\;((\Lambda X_{1}.e_{M})\;\lbrace X_{2}\rbrace))]$


\end{case}
\begin{case}
$\mathscr{E}[^{T_{1}\rightarrow T_{2}}HM^{T_{1}\rightarrow T_{2}}\;(\lambda x_{1}:T_{1}.e_{M})]_{H}\rightarrow\mathscr{E}[\lambda x_{2}:T_{1}.(^{T_{2}}HM^{T_{2}}\;((\lambda x_{1}:T_{1}.e_{M})\;(^{T_{1}}MH^{T_{1}}\;x_{2})))]$

\end{case}
\begin{case}
$\mathscr{E}[^{[T]}HM^{[T]}\;(\mathtt{cons}\;v_{M}^{1}\;v_{M}^{2})]_{H}\rightarrow\mathscr{E}[\mathtt{cons}\;(^{T}HM^{T}\;v_{M}^{1})\;(^{[T]}HM^{[T]}\;v_{M}^{2})]$

\end{case}
\begin{case}
$\mathscr{E}[^{N}HS\;\overline{n}]_{H}\rightarrow\mathscr{E}[\overline{n}]$

\end{case}
\begin{case}
$\mathscr{E}[^{N}HS\;v_{S}]_{H}\rightarrow\mathscr{E}[^{N}HS\;(\mathtt{wrong}\;\mathrm{``Not\;a\;number"})]\;(v_{S}\neq\overline{n}$ for any $\overline{n})$

\end{case}
\begin{case}
$\mathscr{E}[(^{\forall X.T_{1}}HS\;v_{S})\;\lbrace T_{2}\rbrace]_{H}\rightarrow\mathscr{E}[^{T_{1}[T^{a}_{2}/X]}HS\;v_{S}]$

\end{case}
\begin{case}
$\mathscr{E}[^{T_{1}\rightarrow T_{2}}HS\;(\lambda x_{1}.e_{S})]_{H}\rightarrow\mathscr{E}[\lambda x_{2}:T_{1}[T_{i}/T^{a}_{i}].(^{T_{2}}HS\;((\lambda x_{1}.e_{S})\;(SH^{T_{1}}\;x_{2})))]$

\end{case}
\begin{case}
$\mathscr{E}[^{T_{1}\rightarrow T_{2}}HS\;v_{S}]_{H}\rightarrow\mathscr{E}[^{T_{1}\rightarrow T_{2}}HS\;(\mathtt{wrong}\;\mathrm{``Not\;a\;procedure"})]\;(v_{S}\neq\lambda x.e_{S}$ for any $x$ or $e_{S})$

\end{case}
\begin{case}
$\mathscr{E}[^{T^{a}}HS\;(SH^{T^{a}}\;e_{H})]_{H}\rightarrow\mathscr{E}[e_{H}]$

\end{case}
\begin{case}
$\mathscr{E}[^{T^{a}}HS\;v_{S}]_{H}\rightarrow\mathscr{E}[^{T^{a}}HS\;(\mathtt{wrong}\;\mathrm{``Parametricity\;violated"})]\;(v_{S}\neq SH^{T^{a}}\;e_{H}$ for any $e_{H})$

\end{case}
\begin{case}
$\mathscr{E}[^{[T]}HS\;(\mathtt{cons}\;v_{S}^{1}\;v_{S}^{2})]_{H}\rightarrow\mathscr{E}[\mathtt{cons}\;(^{T}HS\;v_{S}^{1})\;(^{[T]}HS\;v_{S}^{2})]$

\end{case}
\begin{case}
$\mathscr{E}[^{[T]}HS\;v_{S}^{1}]_{H}\rightarrow\mathscr{E}[^{[T]}HS\;(\mathtt{wrong}\;\mathrm{``Not\;a\;list"})]\;(v_{S}^{1}\neq\mathtt{cons}\;v_{S}^{2}\;v_{S}^{3}$ for any $v_{S}^{2}$ or $v_{S}^{3})$

\end{case}
\end{proof}
\end{theorem}