\begin{case}

$e_{M}=\mathtt{cons}$ $e_{M}^{1}$ $e_{M}^{2}$

$e_{M}^{1}$ is a value or $e_{M}^{1}\rightarrow e_{M}^{3}$ or $e_{M}^{1}\rightarrow$ \emph{\textbf{Error}: string} by the induction hypothesis.  If $e_{M}^{1}\rightarrow e_{M}^{3}$ then $\mathtt{cons}$ $e_{M}^{1}$ $e_{M}^{2}\rightarrow\mathtt{cons}$ $e_{M}^{3}$ $e_{M}^{2}$.  If $e_{M}^{1}\rightarrow$ \emph{\textbf{Error}: string} then $\mathtt{cons}$ $e_{M}^{1}$ $e_{M}^{2}\rightarrow$ \emph{\textbf{Error}: string}.  $e_{M}^{2}$ is a value or $e_{M}^{2}\rightarrow e_{M}^{4}$ or $e_{M}^{2}\rightarrow$ \emph{\textbf{Error}: string} by the induction hypothesis.  If $e_{M}^{2}\rightarrow e_{M}^{4}$ and $e_{M}^{1}$ is a value then $\mathtt{cons}$ $e_{M}^{1}$ $e_{M}^{2}\rightarrow\mathtt{cons}$ $e_{M}^{1}$ $e_{M}^{4}$.  If $e_{M}^{2}\rightarrow$ \emph{\textbf{Error}: string} and $e_{M}^{1}$ is a value then $\mathtt{cons}$ $e_{M}^{1}$ $e_{M}^{2}\rightarrow$ \emph{\textbf{Error}: string}.  If $e_{M}^{1}$ and $e_{M}^{2}$ are values then $\mathtt{cons}$ $e_{M}^{1}$ $e_{M}^{2}$ is a value.

\end{case}