\begin{case}

$e_{H}={^{T}H}M^{T}$ $e_{M}^{1}$

$e_{M}^{1}$ is a value or $e_{M}^{1}\rightarrow e_{M}^{2}$ or $e_{M}^{1}\rightarrow$ \emph{\textbf{Error}: string} by the induction hypothesis.  If $e_{M}^{1}\rightarrow e_{M}^{2}$ then $^{T}HM^{T}$ $e_{M}^{1}\rightarrow{^{T}H}M$ $e_{M}^{2}$.  If $e_{M}^{1}\rightarrow$ \emph{\textbf{Error}: string} then $^{T}HM^{T}$ $e_{M}^{1}\rightarrow$ \emph{\textbf{Error}: string}.  If $e_{M}^{1}$ is a value then $T$ determines the reduction of $^{T}HM^{T}$ $e_{M}^{1}$:

\begin{subcase}

$T=L$

$e_{M}^{1}={^{L}M}S$ $v_{S}$ by canonical forms (Lemma \ref{cf}).  $^{L}HM^{L}$ $(^{L}MS$ $v_{S})\rightarrow{^{L}H}S$ $v_{S}$.

\end{subcase}

\begin{subcase}

$T=N$

$e_{M}^{1}=\overline{n}$ by canonical forms (Lemma \ref{cf}).  $^{N}HM^{N}$ $\overline{n}\rightarrow\overline{n}$.

\end{subcase}

\begin{subcase}

$T=[T_{1}]$

$e_{M}^{1}\in\lbrace\mathtt{nil}^{T_{1}},\mathtt{cons}$ $v_{M}^{1}$ $v_{M}^{2},{^{[T_{1}]}M}H^{[T_{1}]}$ $(\mathtt{cons}$ $e_{H}^{1}$ $e_{H}^{2})\rbrace$ by canonical forms (Lemma \ref{cf}).  $^{[T_{1}]}HM^{[T_{1}]}$ $\mathtt{nil}^{T}\rightarrow\mathtt{nil}^{T}$.  $^{[T_{1}]}HM^{[T_{1}]}$ $(\mathtt{cons}$ $v_{M}^{1}$ $v_{M}^{2})\rightarrow\mathtt{cons}$ $(^{T_{1}}HM^{T_{1}}$ $v_{M}^{1})$ $(^{[T_{1}]}HM^{[T_{1}]}$ $v_{M}^{2})]$.  $^{[T_{1}]}HM^{[T_{1}]}$ $(^{[T_{1}]}MH^{[T_{1}]}$ $(\mathtt{cons}$ $e_{H}^{1}$ $e_{H}^{2}))\rightarrow\mathtt{cons}$ $e_{H}^{1}$ $e_{H}^{2}$.

\end{subcase}

\begin{subcase}

$T=T_{1}^{a}$

Cannot occur because $T_{1}^{a}$ occurs only in $^{T_{1}^{a}}HS$ $e_{S}$.

\end{subcase}

\begin{subcase}

$T=T_{1}\rightarrow T_{2}$

$e_{M}^{1}=\lambda x_{1}:T_{1}.e_{M}^{2}$ by canonical forms (Lemma \ref{cf}).  $^{T_{1}\rightarrow T_{2}}HM^{T_{1}\rightarrow T_{2}}$ $(\lambda x_{1}:T_{1}.e_{M}^{2})\rightarrow\lambda x_{2}:T_{1}.(^{T_{2}}HM^{T_{2}}$ $((\lambda x_{1}:T_{1}.e_{M}^{2})$ $(^{T_{1}}MH^{T_{1}}$ $x_{2})))$.

\end{subcase}

\begin{subcase}

$T=\forall X.T_{1}$

$e_{M}^{1}\in\lbrace\Lambda X.e_{M}^{2},{^{\forall X.T_{1}}M}S$ $v_{S}\rbrace$ by canonical forms (Lemma \ref{cf}).  $^{\forall X.T_{1}}HM^{\forall X.T_{1}}$ $(\Lambda X.e_{M}^{2})\rightarrow\Lambda X.(^{T_{1}}HM^{T_{1}}$ $e_{M}^{2})$.  $^{\forall X.T_{1}}HM^{\forall X.T_{1}}$ $(^{\forall X.T_{1}}MS$ $v_{S})\rightarrow{^{\forall X.T_{1}}H}S$ $v_{S}$.

\end{subcase}

\end{case}