\begin{figure}[p]
\centering
\begin{tabular}{l}

$\mathscr{E}[(\lambda x^h:t.e^h_1)$ $e^h_2]^h\rightarrow\mathscr{E}[e^h_1[e^h_2/x^h]]$ \\

$\mathscr{E}[(\Lambda x^h.e^h)$ $\lbrace t\rbrace]^h\rightarrow\mathscr{E}[e^h[t/x^h]]$ \\

$\mathscr{E}[\mathtt{fix}$ $(\lambda x^h:t.e^h)]^h\rightarrow\mathscr{E}[e^h[(\mathtt{fix}$ $(\lambda x^h:t.e^h))/x^h]]$ \\

$\mathscr{E}[+$ $\overline{n_1}$ $\overline{n_2}]^h\rightarrow\mathscr{E}[\overline{n_1+n_2}]$ \\

$\mathscr{E}[-$ $\overline{n_1}$ $\overline{n_2}]^h\rightarrow\mathscr{E}[\overline{max(n_1-n_2,0)}]$ \\

$\mathscr{E}[\mathtt{if0}$ $\overline{0}$ $e^h_1$ $e^h_2]^h\rightarrow\mathscr{E}[e^h_1]$ \\

$\mathscr{E}[\mathtt{if0}$ $\overline{n}$ $e^h_1$ $e^h_2]^h\rightarrow\mathscr{E}[e^h_2]$ $(n\neq0)$ \\

$\mathscr{E}[\mathtt{hd}$ $(\mathtt{nil}\;t)]^h\rightarrow\mathscr{E}[\mathtt{wrong}\;t$ ``Empty list"$]$ \\

$\mathscr{E}[\mathtt{tl}$ $(\mathtt{nil}\;t)]^h\rightarrow\mathscr{E}[\mathtt{wrong}\;[t]$ ``Empty list"$]$ \\

$\mathscr{E}[\mathtt{hd}$ $(\mathtt{cons}$ $e^h_1$ $e^h_2)]^h\rightarrow\mathscr{E}[e^h_1]$ \\

$\mathscr{E}[\mathtt{tl}$ $(\mathtt{cons}$ $e^h_1$ $e^h_2)]^h\rightarrow\mathscr{E}[e^h_2]$ \\

$\mathscr{E}[\mathtt{null?}$ $(\mathtt{nil}\;t)]^h\rightarrow\mathscr{E}[\overline{0}]$ \\

$\mathscr{E}[\mathtt{null?}$ $(\mathtt{cons}$ $e^h_1$ $e^h_2)]^h\rightarrow\mathscr{E}[\overline{1}]$ \\

$\mathscr{E}[\mathtt{wrong}\;t$ string$]^h\rightarrow$ \textbf{Error}: string

\end{tabular}
\caption{Haskell operational semantics}
\label{hos}
\end{figure}