\begin{figure}[p]
\centering
\begin{tabular}{l}

% hm t (mh t e)

$\mathscr{E}[\mathtt{hm}$ $t$ $(\mathtt{mh}$ $t$ $e^h)]^h\rightarrow\mathscr{E}[e^h]$ \\

% hm L (ms L v)

$\mathscr{E}[\mathtt{hm}$ $\mathtt{L}$ $(\mathtt{ms}$ $\mathtt{L}$ $v^s)]^h\rightarrow\mathscr{E}[\mathtt{hs}$ $\mathtt{L}$ $v^s]$ \\

% hm N n

$\mathscr{E}[\mathtt{hm}$ $\mathtt{N}$ $\overline{n}]^h\rightarrow\mathscr{E}[\overline{n}]$ \\

% hm [t] (nil t)

$\mathscr{E}[\mathtt{hm}$ $[t]$ $(\mathtt{nil}$ $t)]^h\rightarrow\mathscr{E}[\mathtt{nil}$ $t]$ \\

% hm [t] (cons v v)

$\mathscr{E}[\mathtt{hm}$ $[t]$ $(\mathtt{cons}$ $v^m_1$ $v^m_2)]^h\rightarrow\mathscr{E}[\mathtt{cons}$ $(\mathtt{hm}$ $t$ $v^m_1)$ $(\mathtt{hm}$ $[t]$ $v^m_2)]$ \\

% hm (t -> t) (\ x : t . e)

$\mathscr{E}[\mathtt{hm}$ $(t_1\rightarrow t_2)$ $(\lambda x^m:t_1.e^m)]^h\rightarrow\mathscr{E}[\lambda x^h:t_1.(\mathtt{hm}$ $t_2$ $((\lambda x^m:t_1.e^m)$ $(\mathtt{mh}$ $t_1$ $x^h)))]$ \\

% hm (A x . t) (\\ x . e)

$\mathscr{E}[\mathtt{hm}$ $(\forall x^h.t)$ $(\Lambda x^m.e^m)]^h\rightarrow\mathscr{E}[\Lambda x^h.\mathtt{hm}$ $t$ $e^m]$ \\

% hm (A x . t) (ms (A x . t) v)

$\mathscr{E}[\mathtt{hm}$ $(\forall x^h.t)$ $(\mathtt{ms}$ $(\forall x^h.t)$ $v^s)]^h\rightarrow\mathscr{E}[\mathtt{hs}$ $(\forall x^h.t)$ $v^s]$ \\

\end{tabular}
\caption{Haskell-ML operational semantics}
\label{hmos}
\end{figure}