\begin{figure}
\centering
\begin{tabular}{ll}
\vspace{5pt}

& $((((^{\forall X_{1}.(\forall X_{2}.(X_{1}\rightarrow(X_{2}\rightarrow X_{2})))}HS$ $\lambda x_{1}.(\lambda x_{2}.x_{1}))$ $\lbrace N\rbrace)$ $\lbrace N\rbrace)$ $\overline{0})$ $\overline{1}$ \\

\vspace{5pt}

$\rightarrow$ & $(((^{\forall X_{2}.(N^{a}\rightarrow(X_{2}\rightarrow X_{2}))}HS$ $\lambda x_{1}.(\lambda x_{2}.x_{1}))$ $\lbrace N\rbrace)$ $\overline{0})$ $\overline{1}$ \\

\vspace{5pt}

$\rightarrow$ & $((^{N^{a}\rightarrow(N^{b}\rightarrow N^{b}))}HS$ $\lambda x_{1}.(\lambda x_{2}.x_{1}))$ $\overline{0})$ $\overline{1}$ \\

\vspace{5pt}

$\rightarrow$ & $((\lambda x_{3}:N.(^{N^{b}\rightarrow N^{b}}HS$ $((\lambda x_{1}.(\lambda x_{2}.x_{1}))$ $(SH^{N^{a}}$ $x_{3}))))$ $\overline{0})$ $\overline{1}$ \\

\vspace{5pt}

$\rightarrow$ & $(^{N^{b}\rightarrow N^{b}}HS$ $((\lambda x_{1}.(\lambda x_{2}.x_{1}))$ $(SH^{N^{a}}$ $\overline{0})))$ $\overline{1}$ \\

\vspace{5pt}

$\rightarrow$ & $(\lambda x_{4}:N.(^{N^{b}}HS$ $(((\lambda x_{1}.(\lambda x_{2}.x_{1}))$ $(SH^{N^{a}}$ $\overline{0}))$ $(SH^{N^{b}}$ $x_{4}))))$ $\overline{1}$ \\

\vspace{5pt}

$\rightarrow$ & ${^{N^{b}}H}S$ $(((\lambda x_{1}.(\lambda x_{2}.x_{1}))$ $(SH^{N^{a}}$ $\overline{0}))$ $(SH^{N^{b}}$ $\overline{1}))$ \\

\vspace{5pt}

$\rightarrow$ & ${^{N^{b}}H}S$ $((\lambda x_{2}.(SH^{N^{a}}$ $\overline{0}))$ $(SH^{N^{b}}$ $\overline{1}))$ \\

\vspace{5pt}

$\rightarrow$ & ${^{N^{b}}H}S$ $(SH^{N^{a}}$ $\overline{0})$ \\

\vspace{5pt}

$\rightarrow$ & $\mathtt{wrong}$ ``Parametricity violated" \\

\vspace{5pt}

$\rightarrow$ & \textbf{Error}: ``Parametricity violated"
\end{tabular}
\caption{Scheme breaking parametricity}
\label{parametricity-example-2}
\end{figure}