\begin{figure}[p]
\centering
\begin{tabular}{l}

$\mathscr{E}[\mathtt{sh}$ $\mathtt{L}$ $(\mathtt{hs}$ $\mathtt{L}$ $v^s)]^s\rightarrow\mathscr{E}[v^s]$ \\

$\mathscr{E}[\mathtt{sh}$ $\mathtt{N}$ $\overline{n}]^s\rightarrow\mathscr{E}[\overline{n}]$ \\

$\mathscr{E}[\mathtt{sh}$ $[t]$ $(\mathtt{nil}$ $t[t_i/t_i.x^h])]^s\rightarrow\mathscr{E}[\mathtt{nil}]$ \\

$\mathscr{E}[\mathtt{sh}$ $[t]$ $(\mathtt{cons}$ $e^h_1$ $e^h_2)]^s\rightarrow\mathscr{E}[\mathtt{cons}$ $(\mathtt{sh}$ $t$ $e^h_1)$ $(\mathtt{sh}$ $[t]$ $e^h_2)]$ \\

$\mathscr{E}[\mathtt{sh}$ $(t_1\rightarrow t_2)$ $(\lambda x^h:t_1[t_i/t_i.x^h].e^h)]^s\rightarrow$ \\

$\quad\quad\mathscr{E}[\lambda x^s.\mathtt{sh}$ $t_2$ $((\lambda x^h:t_1[t_i/t_i.x^h].e^h)$ $(\mathtt{hs}$ $t_1$ $x^s))]$ \\

$\mathscr{E}[\mathtt{sh}$ $(\forall x^h.t)$ $(\Lambda x^h.e^h)]^s\rightarrow\mathscr{E}[\mathtt{sh}$ $t[\mathtt{L}/x^h]$ $e^h[\mathtt{L}/x^h]]$ \\

$\mathscr{E}[\mathtt{sh}$ $(\forall x^h.t)$ $(\mathtt{hs}$ $(\forall x^h.t)$ $v^s)]^s\rightarrow\mathscr{E}[v^s]$ \\

\end{tabular}
\caption{Scheme-Haskell operational semantics}
\label{shos}
\end{figure}